updated propLogic to match workshop goals

GlimpseOfLean/Exercises/Topics/ClassicalPropositionalLogic.lean
@@ -3,39 +3,42 @@ open Set
 
 namespace ClassicalPropositionalLogic
 
-/- Let's try to implement a language of classical propositional logic.
-
-Note that there is also version of this file for intuitionistic logic:
-`IntuitionisticPropositionalLogic.lean`
+/- Let's try to implement a language of classical propositional logic
 -/
 
 def Variable : Type := ℕ
 
-/- We define propositional formula, and some notation for them. -/
-
+/- We define the notion of propositional `Formula` inductively.
+    The base cases consist of variable, indexed by the `Variable` type defined above, or the falsum.
+    New formulas are made through conjunction, disjunction and implication.
+    The negation `~A` of a formula `A` is defined as `A ⇒ bot`, see below. -/
 inductive Formula : Type where
-  | var : Variable → Formula
-  | bot : Formula
+  | var : Variable → Formula -- indexed variable symbols
+  | bot : Formula -- the falsum
   | conj : Formula → Formula → Formula
   | disj : Formula → Formula → Formula
-  | impl : Formula → Formula → Formula
+  | imp : Formula → Formula → Formula
 
+/- We define some notation. Recall that you can mouse over a symbol to see how to write it. -/
 open Formula
 local notation:max (priority := high) "#" x:max => var x
 local infix:30 (priority := high) " || " => disj
 local infix:35 (priority := high) " && " => conj
-local infix:28 (priority := high) " ⇒ " => impl
+local infix:28 (priority := high) " ⇒ " => imp
 local notation (priority := high) "⊥" => bot
 
 def neg (A : Formula) : Formula := A ⇒ ⊥
 local notation:(max+2) (priority := high) "~" x:max => neg x
+
 def top : Formula := ~⊥
 local notation (priority := high) "⊤" => top
+
 def equiv (A B : Formula) : Formula := (A ⇒ B) && (B ⇒ A)
 local infix:29 (priority := high) " ⇔ " => equiv
 
-/- Let's define truth w.r.t. a valuation, i.e. classical validity -/
-
+/- Given an evaluation to `True` or `False` for each variable symbol,
+  we can inductively define "truth" (with respect to Lean's underlying logic)
+  of arbitrary propositional formulas. -/
 @[simp]
 def IsTrue (φ : Variable → Prop) : Formula → Prop
   | ⊥      => False
@@ -44,35 +47,54 @@ def IsTrue (φ : Variable → Prop) : Formula → Prop
   | A && B => IsTrue φ A ∧ IsTrue φ B
   | A ⇒ B => IsTrue φ A → IsTrue φ B
 
+/-- A set of Formulas is satisfied if every element evaluates to `True`-/
 def Satisfies (φ : Variable → Prop) (Γ : Set Formula) : Prop := ∀ {A}, A ∈ Γ → IsTrue φ A
+
+/-- A formula `A` is modeled by a theory (= Set of formulas) `Γ` if `A` holds
+  whenever `Γ` is satisfied. -/
 def Models (Γ : Set Formula) (A : Formula) : Prop := ∀ {φ}, Satisfies φ Γ → IsTrue φ A
+
 local infix:27 (priority := high) " ⊨ " => Models
+
+/-- If a formula is modeled by the empty theory, then it is a valid formula. -/
 def Valid (A : Formula) : Prop := ∅ ⊨ A
 
-/- Here are some basic properties of validity.
-
-  The tactic `simp` will automatically simplify definitions tagged with `@[simp]` and rewrite
-  using theorems tagged with `@[simp]`. -/
-
 variable {φ : Variable → Prop} {A B : Formula}
-@[simp] lemma isTrue_neg : IsTrue φ ~A ↔ ¬ IsTrue φ A := by simp [neg]
+
+/- We record some lemmas below that are not strictly necessary.
+  They help to rewrite the more syntactic left-hand side to the more  semantic right-hand side.
+  This may be helpful when exploring proof strategies. -/
+lemma isTrue_bot : IsTrue φ ⊥ ↔ False := Iff.rfl
+
+lemma isTrue_var {P} : IsTrue φ (# P) ↔ φ P := Iff.rfl
+
+lemma isTrue_or : IsTrue φ (A || B) ↔ IsTrue φ A ∨ IsTrue φ B := Iff.rfl
+
+lemma isTrue_and : IsTrue φ (A && B) ↔ IsTrue φ A ∧ IsTrue φ B := Iff.rfl
+
+lemma isTrue_imp : IsTrue φ (A ⇒ B) ↔ IsTrue φ A → IsTrue φ B := Iff.rfl
+
+/- Here are some basic properties of validity.
+We tag these lemmas with `@[simp]` so that they are automatically used by the `simp` tactic. -/
+@[simp] lemma isTrue_neg : IsTrue φ ~A ↔ ¬ IsTrue φ A := by
+  sorry
+
 
 @[simp] lemma isTrue_top : IsTrue φ ⊤ := by
   sorry
 
+
 @[simp] lemma isTrue_equiv : IsTrue φ (A ⇔ B) ↔ (IsTrue φ A ↔ IsTrue φ B) := by
   sorry
 
-/- As an exercise, let's prove (using classical logic) the double negation elimination principle.
-  `by_contra h` might be useful to prove something by contradiction. -/
-
+/- As an exercise, let's prove (using classical logic) the double negation elimination principle. -/
 example : Valid (~~A ⇔ A) := by
   sorry
 
+
 /- We will frequently need to add an element to a set. This is done using
 the `insert` function: `insert A Γ` means `Γ ∪ {A}`. -/
-
-@[simp] lemma satisfies_insert_iff : Satisfies φ (insert A Γ) ↔ IsTrue φ A ∧ Satisfies φ Γ := by
+@[simp] lemma satisfies_insert_iff {Γ} : Satisfies φ (insert A Γ) ↔ IsTrue φ A ∧ Satisfies φ Γ := by
   simp [Satisfies]
 
 /- Let's define provability w.r.t. classical logic. -/
@@ -83,14 +105,19 @@ local infix:27 " ⊢ " => ProvableFrom
 /- `Γ ⊢ A` is the predicate that there is a proof tree with conclusion `A` with assumptions from
   `Γ`. This is a typical list of rules for natural deduction with classical logic. -/
 inductive ProvableFrom : Set Formula → Formula → Prop
+  -- `A` belongs to the list of axioms
   | ax    : ∀ {Γ A},   A ∈ Γ   → Γ ⊢ A
+  -- If we can prove `B` from `Γ ∪ {a}`, then `Γ ⊢ A ⇒ B`
   | impI  : ∀ {Γ A B},  insert A Γ ⊢ B                → Γ ⊢ A ⇒ B
-  | impE  : ∀ {Γ A B},           Γ ⊢ (A ⇒ B) → Γ ⊢ A  → Γ ⊢ B
+  /- If we have a proof that `A ⇒ B` also of `A`, then obtain a proof of `B`.
+    The variable `A` is made explicit here to help get more context from the Lean InfoView. -/
+  | impE  : ∀ {Γ B} (A),           Γ ⊢ (A ⇒ B) → Γ ⊢ A  → Γ ⊢ B
   | andI  : ∀ {Γ A B},           Γ ⊢ A       → Γ ⊢ B  → Γ ⊢ A && B
   | andE1 : ∀ {Γ A B},           Γ ⊢ A && B           → Γ ⊢ A
   | andE2 : ∀ {Γ A B},           Γ ⊢ A && B           → Γ ⊢ B
   | orI1  : ∀ {Γ A B},           Γ ⊢ A                → Γ ⊢ A || B
   | orI2  : ∀ {Γ A B},           Γ ⊢ B                → Γ ⊢ A || B
+  -- Recall that `insert A Γ` means `Γ ∪ {A}`
   | orE   : ∀ {Γ A B C}, Γ ⊢ A || B → insert A Γ ⊢ C → insert B Γ ⊢ C → Γ ⊢ C
   | botC  : ∀ {Γ A},   insert ~A Γ ⊢ ⊥                → Γ ⊢ A
 
@@ -102,9 +129,25 @@ local infix:27 (priority := high) " ⊢ " => ProvableFrom
 def Provable (A : Formula) := ∅ ⊢ A
 
 export ProvableFrom (ax impI impE botC andI andE1 andE2 orI1 orI2 orE)
-variable {Γ Δ : Set Formula}
+variable {Γ : Set Formula}
 
-/- We define a simple tactic `apply_ax` to prove something using the `ax` rule. -/
+/- Proving something using the ax rule requires showing that `A ∈ Γ`. In the concrete situations we
+  will encounter, the following lemmas about insert will suffice most of the time.
+  ```
+  mem_singleton x : x ∈ {x}
+  mem_insert x s : x ∈ insert x s
+  mem_insert_of_mem y : x ∈ s → x ∈ insert y s
+  ```
+  -/
+
+/- Prove the following using the above lemmas about `insert`-/
+example : {A, B} ⊢ A && B := by sorry
+
+
+/- Arguments as above can become pretty tedious.
+  We define a simple tactic `apply_ax`: it proves statements that can be shwon from the ax rule,
+  combined with the three lemmas above
+     -/
 syntax "solve_mem" : tactic
 syntax "apply_ax" : tactic
 macro_rules
@@ -114,38 +157,22 @@ macro_rules
                     | fail "tactic \'apply_ax\' failed")
   | `(tactic| apply_ax)  => `(tactic| { apply ax; solve_mem })
 
-/- To practice with the proof system, let's prove the following.
-  You can either use the `apply_ax` tactic defined on the previous lines, which proves a goal that
-  is provable using the `ax` rule.
-  Or you can do it manually, using the following lemmas about insert.
-```
-  mem_singleton x : x ∈ {x}
-  mem_insert x s : x ∈ insert x s
-  mem_insert_of_mem y : x ∈ s → x ∈ insert y s
-```
--/
+-- Now use the `apply_ax` tactic to show the same example
+example : {A, B} ⊢ A && B := by sorry
 
--- Let’s first see an example using the `apply_ax` tactic
-example : {A, B} ⊢ A && B := by
-  apply andI
-  apply_ax
-  apply_ax
 
--- And the same one done by hand in one go.
-example : {A, B} ⊢ A && B := by
-  exact andI (ax (mem_insert _ _)) (ax (mem_insert_of_mem _ (mem_singleton _)))
-
+/- All of the below examples can be completed by a chain of `apply (proofRule)` statements, combined
+  with our custom `apply_ax` tactic. -/
 
 example : Provable (~~A ⇔ A) := by
   sorry
 
 /- Optional exercise: prove the law of excluded middle. -/
 example : Provable (A || ~A) := by
-  sorry
+ sorry
 
 /- Optional exercise: prove one of the de-Morgan laws.
-  If you want to say that the argument called `A` of the axiom `impE` should be `X && Y`,
-  you can do this using `impE (A := X && Y)` -/
+  This is a bit more work than the previous ones -/
 example : Provable (~(A && B) ⇔ ~A || ~B) := by
   sorry
 
@@ -157,12 +184,14 @@ example : Provable (~(A && B) ⇔ ~A || ~B) := by
   `rename_i A B h ih`. Or you can prove a particular case using `case impI ih => <proof>`.
   You will probably need to use the lemma
   `insert_subset_insert : s ⊆ t → insert x s ⊆ insert x t`. -/
-lemma weakening (h : Γ ⊢ A) (h2 : Γ ⊆ Δ) : Δ ⊢ A := by
+lemma weakening {Δ : Set Formula} (h : Γ ⊢ A) (h2 : Γ ⊆ Δ) : Δ ⊢ A := by
+  sorry
+
+lemma weakening' {Δ} (h : Γ ⊢ A) (h2 : Γ ⊆ Δ) : Δ ⊢ A := by
   sorry
 
 /- Use the `apply?` tactic to find the lemma that states `Γ ⊆ insert x Γ`.
   You can click the blue suggestion in the right panel to automatically apply the suggestion. -/
-
 lemma ProvableFrom.insert (h : Γ ⊢ A) : insert B Γ ⊢ A := by
   sorry
 
@@ -173,18 +202,22 @@ lemma deduction_theorem (h : Γ ⊢ A) : insert (A ⇒ B) Γ ⊢ B := by
 lemma Provable.mp (h1 : Provable (A ⇒ B)) (h2 : Γ ⊢ A) : Γ ⊢ B := by
   sorry
 
-/-- You will want to use the tactics `left` and `right` to prove a disjunction, and the
-  tactic `cases h` if `h` is a disjunction to do a case distinction. -/
+/-- To prove a disjunction, you can use the tactics `left` and `right`, or directly use
+  the constructors `Or.inl` and `Or.inr`.
+  To eliminate from a disjunction `h`, you can use `cases h` and obtain cases `inl a` and `inr b`. -/
 theorem soundness_theorem (h : Γ ⊢ A) : Γ ⊨ A := by
+  sorry
+
+theorem soundness_theorem' (h : Γ ⊢ A) : Γ ⊨ A := by
   sorry
 
 theorem valid_of_provable (h : Provable A) : Valid A := by
   sorry
 
-/-
-  If you want, you can now try some these longer projects.
 
-  1. Prove completeness: if a formula is valid, then it is provable
+/-
+  If you want, you can now try to prove completeness: if a formula is valid, then it is provable
+
   Here is one possible strategy for this proof:
   * If a formula is valid, then so is its negation normal form (NNF);
   * If a formula in NNF is valid, then so is its conjunctive normal form (CNF);
@@ -193,10 +226,8 @@ theorem valid_of_provable (h : Provable A) : Valid A := by
   * If a formula in CNF is syntactically valid, then its provable;
   * If the CNF of a formula in NNF is provable, then so is the formula itself.
   * If the NNF of a formula is provable, then so is the formula itself.
-
-  2. Define Gentzen's sequent calculus for propositional logic, and prove that this gives rise
-  to the same provability.
 -/
 
-end ClassicalPropositionalLogic
 
+
+end ClassicalPropositionalLogic
